\setlength{\parindent}{0pt}

ベルヌーイ分布
\begin{equation*}
  p_X(x)=
  \begin{cases}
    p^x(1-p)^{1-x} & (x=0,1)\\
    0 & (x\neq 0,x\neq 1) \\
  \end{cases}
\end{equation*}
分布関数
\begin{equation*}
  F_X(t)=
  \begin{cases}
    0 & (t < 0) \\
    1-p & (0 \le t < 1) \\
    1 & (t \ge 1) \\
  \end{cases}
\end{equation*}
期待値
\begin{equation*}
  E(X)=0\times (1-p)+1\times p=p \\
\end{equation*}
分散
\begin{equation*}
  V(X)=(0-p)^2(1-p)+(1-p)^2p=p^2-p^3+p-2p^2+p^3=p(1-p) \\
\end{equation*}

二項分布
\begin{equation*}
  p_X(x)=\binom{n}{x}p^x(1-p)^{n-x} (x=0,1,\dots n) \\
\end{equation*}
二項定理
\begin{equation*}
  (a+b)^n=\sum_{x=0}^{n}\binom{n}{x}a^xb^{n-x} \\
\end{equation*}
\begin{equation*}
  \sum_{x}p_X(x)=(p+(1-p))^n=1 \\
\end{equation*}
期待値
\begin{align*}
  E(X)&=\sum_{x=0}^{n}x\binom{n}{x}p^x(1-p)^{n-x} \\
  &=\sum_{x=1}^{n}n\binom{n-1}{x-1}p^x(1-p)^{n-x} \\
  &=np\sum_{x=1}^{n}\binom{n-1}{x-1}p^{x-1}(1-p)^{n-x} \\
  &=np\sum_{x=0}^{n-1}\binom{n-1}{x}p^x(1-p)^{n-x-1} (x\rightarrow x+1) \\
  &=np \\
\end{align*}
分散
\begin{align*}
  V(X)&=\left(\sum_{x=0}^{n}x^2p_X(x)\right)-2\mu\left(\sum_{x=0}^{n}xp_X(x)\right)+\mu^2\left(\sum_{x=0}^{n}p_X(x)\right) \\
  &=\left(\sum_{x=0}^{n}x^2p_X(x)\right)-\mu^2 \\
\end{align*}
\begin{align*}
  \sum_{x=0}^{n}x^2p_X(x)&=\left(\sum_{x=2}^{n}x(x-1)\binom{n}{x}p^x(1-p)^{n-x}\right)+E(X) \\
  &=n(n-1)\left(\sum_{x=2}^{n}\binom{x-2}{n-2}p^x(1-p)^{n-x}\right)+np \\
  &=n(n-1)p^2\left(\sum_{x=2}^{n}\binom{x}{n-2}p^x(1-p)^{n-x-2}\right)+np \\
  &=n(n-1)p^2(p+(1-p))^{n-2}+np \\
  &=n(n-1)p^2+np \\
\end{align*}
\begin{align*}
  V(X)&=n(n-1)p^2+np-n^2p^2 \\
  &=np-np^2 \\
  &=np(1-p) \\
\end{align*}